working/composition/event_based_refinement/load_balancer/compositional/abstract_composition/ComposedDistributedSystem.t.dfy
@@ -1,0 +1,110 @@
+include "../shared/Types.t.dfy"
+include "../shared/Host.t.dfy"
+include "ComposedSpec.t.dfy"
+include "ComposedNetwork.t.dfy"
+
+abstract module ComposedDistributedSystem {
+    import opened Types
+    import ComposedSpec: ComposedSpec
+    import ComposedNetwork: ComposedNetwork
+    import HostA: AbstractHost
+    import HostB: AbstractHost
+
+    datatype Constants = Constants(
+        hostsA: seq<HostA.Constants>,
+        hostsB: seq<HostB.Constants>,
+        network: ComposedNetwork.Constants) 
+    {
+        ghost predicate WF() 
+        {
+            && HostA.GroupWFConstants(hostsA)
+            && HostB.GroupWFConstants(hostsB)
+        }
+    }
+
+    datatype Variables = Variables(
+        hostsA: seq<HostA.Variables>,
+        hostsB: seq<HostB.Variables>,
+        network: ComposedNetwork.Variables) 
+    {
+        ghost predicate WF(c: Constants) {
+            && c.WF()
+            && |c.hostsA| == |hostsA|
+            && HostA.GroupWFVariables(c.hostsA, hostsA)
+            && |c.hostsB| == |hostsB|
+            && HostB.GroupWFVariables(c.hostsB, hostsB)
+        }
+    }
+
+    ghost predicate Init(c: Constants, v: Variables) {
+        && v.WF(c)
+        && (forall i :: 0 <= i < |c.hostsA| ==> HostA.Init(c.hostsA[i], v.hostsA[i]))
+        && (forall i :: 0 <= i < |c.hostsB| ==> HostB.Init(c.hostsB[i], v.hostsB[i]))
+        && ComposedNetwork.Init(c.network, v.network)
+    }
+
+    ghost predicate IsEventA(evt: Option<ComposedSpec.Event>)
+
+    ghost function UnwrapEventA(evt: Option<ComposedSpec.Event>) : Option<HostA.Spec.Event>
+        requires IsEventA(evt)
+
+    ghost predicate IsEventB(evt: Option<ComposedSpec.Event>)
+
+    ghost function UnwrapEventB(evt: Option<ComposedSpec.Event>) : Option<HostB.Spec.Event>
+        requires IsEventB(evt)
+
+    ghost predicate IsMessageOpsA(msgOps: ComposedNetwork.MessageOps)
+
+    ghost function UnwrapMessageOpsA(msgOps: ComposedNetwork.MessageOps): HostA.Network.MessageOps
+        requires IsMessageOpsA(msgOps)
+
+    ghost predicate IsMessageOpsB(msgOps: ComposedNetwork.MessageOps)
+
+    ghost function UnwrapMessageOpsB(msgOps: ComposedNetwork.MessageOps): HostB.Network.MessageOps
+        requires IsMessageOpsB(msgOps)
+
+    ghost predicate HostActionA(c: Constants, v: Variables, v': Variables, evt: Option<ComposedSpec.Event>, hostId: nat, msgOps: ComposedNetwork.MessageOps)
+        requires v.WF(c)
+        requires v'.WF(c)
+    {
+        && 0 <= hostId < |v.hostsA|
+        && IsEventA(evt)
+        && IsMessageOpsA(msgOps)
+        && HostA.Next(c.hostsA[hostId], v.hostsA[hostId], v'.hostsA[hostId], UnwrapEventA(evt), UnwrapMessageOpsA(msgOps))
+        && (forall i :: 0 <= i < |v.hostsA| && i != hostId ==> v.hostsA[i] == v'.hostsA[i])
+        && (forall i :: 0 <= i < |v.hostsB| ==> v.hostsB[i] == v'.hostsB[i])
+    }
+
+    ghost predicate HostActionB(c: Constants, v: Variables, v': Variables, evt: Option<ComposedSpec.Event>, hostId: nat, msgOps: ComposedNetwork.MessageOps)
+        requires v.WF(c)
+        requires v'.WF(c)
+    {
+        && 0 <= hostId < |v.hostsB|
+        && IsEventB(evt)
+        && IsMessageOpsB(msgOps)
+        && HostB.Next(c.hostsB[hostId], v.hostsB[hostId], v'.hostsB[hostId], UnwrapEventB(evt), UnwrapMessageOpsB(msgOps))
+        && (forall i :: 0 <= i < |v.hostsB| && i != hostId ==> v.hostsB[i] == v'.hostsB[i])
+        && (forall i :: 0 <= i < |v.hostsA| ==> v.hostsA[i] == v'.hostsA[i])
+    }
+
+    ghost predicate HostAction(c: Constants, v: Variables, v': Variables, evt: Option<ComposedSpec.Event>, hostId: nat, msgOps: ComposedNetwork.MessageOps)
+    {
+        && v.WF(c)
+        && v'.WF(c)
+        && (HostActionA(c, v, v', evt, hostId, msgOps) || HostActionB(c, v, v', evt, hostId, msgOps))
+        && ComposedNetwork.Next(c.network, v.network, v'.network, msgOps)
+    }
+
+    datatype Step =
+        | HostActionStep(hostId: nat, msgOps: ComposedNetwork.MessageOps)
+
+    ghost predicate NextStep(c: Constants, v: Variables, v': Variables, evt: Option<ComposedSpec.Event>, step: Step)
+    {
+        && HostAction(c, v, v', evt, step.hostId, step.msgOps)
+    }
+
+    ghost predicate Next(c: Constants, v: Variables, v': Variables, evt: Option<ComposedSpec.Event>)
+    //{
+    //    exists step :: NextStep(c, v, v', evt, step)
+    //}
+}
