working/composition/event_based_refinement/load_balancer/compositional/abstract_composition/ComposedHost.t.dfy
@@ -1,0 +1,37 @@
+// include "../shared/Types.t.dfy"
+// include "../shared/Host.t.dfy"
+// include "ComposedSpec.t.dfy"
+// include "ComposedNetwork.t.dfy"
+
+// abstract module ComposedHost {
+//     import opened Types
+//     import Network: ComposedNetwork
+//     import HostImpl: AbstractHost
+//     import opened Spec = HostImpl.Spec
+
+//     datatype Constants = Constants(cnsts: HostImpl.Constants) 
+//     {
+//         ghost predicate WF() {
+//             cnsts.WF()
+//         }
+//     }
+
+//     datatype Variables = Variables(vars: HostImpl.Variables)
+//     {
+//         ghost predicate WF(c: Constants) {
+//             vars.WF(c.cnsts)
+//         }
+//     }
+
+//     ghost predicate GroupWFConstants(c: seq<Constants>)
+//     ghost predicate GroupWFVariables(c: seq<Constants>, v: seq<Variables>)
+
+//     ghost predicate Init(c: Constants, v: Variables) {
+//         HostImpl.Init(c.cnsts, v.vars)
+//     }
+
+//     ghost predicate Next(c: Constants, v: Variables, v': Variables, evt: Option<Event>, msgOps: Network.MessageOps)
+//     {
+//         HostImpl.Next(c.cnsts, v.vars, v'.vars, evt, HostImpl.Network.MessageOps(msgOps.recv, msgOps.send))
+//     }
+// }
