working/composition/event_based_refinement/load_balancer/compositional/abstract_composition/ComposedNetwork.t.dfy
@@ -1,0 +1,43 @@
+include "../shared/Types.t.dfy"
+include "../shared/Network.t.dfy"
+include "../shared/Host.t.dfy"
+
+abstract module ComposedNetwork {
+    import opened Types
+    import HostA : AbstractHost
+    import HostB : AbstractHost
+    import NetworkA : HostA.Network
+    import NetworkB : HostB.Network
+
+    datatype Message = MessageA(msgA: NetworkA.Message) | MessageB(msgB: NetworkB.Message)
+    // todo - can we modify this so that this module can still refine AbstractNetwork?
+    datatype MessageOps = MessageOps(recv:Option<Message>, send:Option<Message>, send_trans:Option<Message>)
+
+    // todo - this feels like it belongs somewhere else
+    ghost predicate TranslateAToB(msgA: NetworkA.Message, msgB: NetworkB.Message)
+    ghost predicate TranslateBToA(msgB: NetworkB.Message, msgA: NetworkA.Message)
+
+    ghost predicate Translate(fromMsg: Option<Message>, toMsg: Option<Message>) {
+        match (fromMsg, toMsg)
+        case (Some(MessageA(_)), Some(MessageB(_))) => TranslateAToB(fromMsg.value.msgA, toMsg.value.msgB)
+        case (Some(MessageB(_)), Some(MessageA(_))) => TranslateBToA(fromMsg.value.msgB, toMsg.value.msgA)
+        case _ => false
+    }
+
+    datatype Constants = Constants  // no constants for network
+
+    datatype Variables = Variables(sentMsgs:set<Message>)
+
+    ghost predicate Init(c: Constants, v: Variables)
+    {
+        && v.sentMsgs == {}
+    }
+
+    ghost predicate Next(c: Constants, v: Variables, v': Variables, msgOps: MessageOps)
+    {
+        && (msgOps.recv.Some? ==> msgOps.recv.value in v.sentMsgs)
+        && v'.sentMsgs == v.sentMsgs
+            + (if msgOps.send.None? then {} else { msgOps.send.value })
+            + (if Translate(msgOps.send, msgOps.send_trans) then { msgOps.send_trans.value } else {})
+  }
+}
