working/composition/event_based_refinement/load_balancer/compositional/abstract_composition/ComposedSpec.t.dfy
@@ -1,0 +1,25 @@
+include "../shared/Spec.t.dfy"
+include "../shared/Host.t.dfy"
+
+abstract module ComposedSpec refines AbstractSpec {
+    import HostA : AbstractHost
+    import HostB : AbstractHost
+    import SpecA : HostA.Spec
+    import SpecB : HostB.Spec
+
+    datatype Event = EventA(evtA: SpecA.Event) | EventB(evtB: SpecB.Event)
+
+    datatype Constants = Constants(cnstsA: SpecA.Constants, cnstsB: SpecB.Constants)
+    datatype Variables = Variables(varsA: SpecA.Variables, varsB: SpecB.Variables)
+
+    ghost predicate Init(c: Constants, v: Variables) {
+        && SpecA.Init(c.cnstsA, v.varsA)
+        && SpecB.Init(c.cnstsB, v.varsB)
+    }
+
+    ghost predicate Next(c: Constants, v: Variables, v': Variables, evt: Event) {
+        match evt 
+        case EventA(_) => SpecA.Next(c.cnstsA, v.varsA, v'.varsA, evt.evtA) && v.varsB == v'.varsB
+        case EventB(_) => SpecB.Next(c.cnstsB, v.varsB, v'.varsB, evt.evtB) && v.varsA == v'.varsA
+    }
+}
