working/composition/event_based_refinement/load_balancer/compositional/client/ClientHost.v.dfy
@@ -1,0 +1,73 @@
+include "ClientSpec.t.dfy"
+include "Network.v.dfy"
+include "../shared/Host.t.dfy"
+
+module ClientHost refines AbstractHost {
+    import opened Spec = ClientSpec
+    import Network = ClientNetwork
+
+    datatype Constants = Constants
+    {
+        ghost predicate WF() {
+            true
+        }
+    }
+
+    datatype Variables = Variables(requests: seq<ServiceRequest<(int, int)>>, responses: seq<ServiceResponse<int>>)
+    {
+        ghost predicate WF(c: Constants) {
+            && |requests| >= |responses|
+            && (forall i :: 0 <= i < |requests| ==> requests[i].seqNo == i)
+            && (forall i :: 0 <= i < |responses| ==> responses[i].seqNo == i)
+        }
+    }
+
+    ghost predicate GroupWFConstants(c: seq<Constants>) 
+    {
+        && |c| == 1
+    }
+
+    ghost predicate GroupWFVariables(c: seq<Constants>, v: seq<Variables>)
+    {
+        && GroupWFConstants(c)
+        && |v| == |c|
+        && v[0].WF(c[0])
+    }
+
+    ghost predicate Init(c: Constants, v: Variables) {
+        && |v.requests| == 0
+        && |v.responses| == 0
+    }
+
+    ghost predicate SendRequest(c: Constants, v: Variables, v': Variables, evt: Option<Spec.Event>, msgOps: Network.MessageOps) {
+        && v.WF(c)
+        && v'.WF(c)
+        && evt.Some? && evt.value.SendRequest?
+        && v.responses == v'.responses
+        && |v'.requests| == |v.requests| + 1
+        && v'.requests[..|v'.requests| - 1] == v.requests
+        && msgOps.recv.None?
+        && msgOps.send.Some?
+        && msgOps.send.value.ClientRequest?
+        && msgOps.send.value.request == v'.requests[|v'.requests| - 1]
+    }
+
+    ghost predicate ReceiveResponse(c: Constants, v: Variables, v': Variables, evt: Option<Spec.Event>, msgOps: Network.MessageOps) {
+        && v.WF(c)
+        && v'.WF(c)
+        && evt.Some? && evt.value.ReceiveResponse?
+        && v.requests == v'.requests
+        && msgOps.recv.Some?
+        && msgOps.recv.value.ClientResponse?
+        && msgOps.send.None?
+        && |v'.responses| == |v.responses| + 1
+        && v'.responses[..|v'.responses| - 1] == v.responses 
+        && v'.responses[|v'.responses| - 1] == msgOps.recv.value.response
+    }
+
+    ghost predicate Next(c: Constants, v: Variables, v': Variables, evt: Option<Spec.Event>, msgOps: Network.MessageOps)
+    {
+        || SendRequest(c, v, v', evt, msgOps) 
+        || ReceiveResponse(c, v, v', evt, msgOps) 
+    }
+}
