working/composition/event_based_refinement/load_balancer/compositional/client/Network.v.dfy
@@ -1,0 +1,6 @@
+include "ClientSpec.t.dfy"
+include "../shared/Network.t.dfy"
+
+module ClientNetwork refines AbstractNetwork {
+    datatype Message = ClientRequest(request: ServiceRequest<(int, int)>) | ClientResponse(response: ServiceResponse<int>)
+}
