working/composition/event_based_refinement/load_balancer/compositional/client/RefinementProof.v.dfy
@@ -1,0 +1,85 @@
+include "../shared/RefinementObligation.t.dfy"
+include "ClientHost.v.dfy"
+include "Network.v.dfy"
+include "DistributedSystem.v.dfy"
+
+module RefinementProof refines RefinementTheorem {
+    import opened DistributedSystem = DistributedSystem
+
+    ghost function ConstantsAbstraction(c: DistributedSystem.Constants) : Host.Spec.Constants
+//        requires c.WF()
+    {
+        Host.Spec.Constants()
+    }
+
+    ghost function MapClientRequests(clientRequests: seq<ServiceRequest<(int, int)>>) : seq<(int, int)>
+        decreases |clientRequests|
+        ensures |clientRequests| == |MapClientRequests(clientRequests)|
+        ensures forall i :: 0 <= i < |clientRequests| ==> MapClientRequests(clientRequests)[i] == (clientRequests[i].val.0, clientRequests[i].val.1)
+    {
+        if |clientRequests| == 0
+            then [] 
+            else [(clientRequests[0].val.0, clientRequests[0].val.1)] + MapClientRequests(clientRequests[1..])
+    }
+
+    ghost function MapClientResponses(clientResponses: seq<ServiceResponse<int>>) : seq<(int)>
+        decreases |clientResponses|
+        ensures |clientResponses| == |MapClientResponses(clientResponses)|
+        ensures forall i :: 0 <= i < |clientResponses| ==> MapClientResponses(clientResponses)[i] == clientResponses[i].val
+    {
+        if |clientResponses| == 0
+            then [] 
+            else [clientResponses[0].val] + MapClientResponses(clientResponses[1..])
+    }
+
+    ghost function VariablesAbstraction(c: DistributedSystem.Constants, v: DistributedSystem.Variables) : Host.Spec.Variables
+//        requires v.WF(c)
+    {
+        Host.Spec.Variables(
+            MapClientRequests(v.hosts[0].requests), 
+            MapClientResponses(v.hosts[0].responses)
+        )
+    }
+
+    ghost predicate Inv_ClientRequestMsg(c: DistributedSystem.Constants, v: DistributedSystem.Variables) 
+        requires v.WF(c)
+    {
+        forall msg :: 
+            && msg in v.network.sentMsgs 
+            && msg.ClientRequest? ==> 
+            && |v.hosts[0].requests| > msg.request.seqNo 
+            && v.hosts[0].requests[msg.request.seqNo] == msg.request
+    }
+
+    ghost predicate Inv_ClientResponseMsg(c: DistributedSystem.Constants, v: DistributedSystem.Variables) 
+        requires v.WF(c)
+    {
+        forall msg :: 
+            && msg in v.network.sentMsgs 
+            && msg.ClientResponse? ==> 
+            && |v.hosts[0].requests| > msg.response.seqNo 
+            && v.hosts[0].requests[msg.response.seqNo].val.0 + v.hosts[0].requests[msg.response.seqNo].val.1 == msg.response.val
+    }
+
+    ghost predicate Inv(c: DistributedSystem.Constants, v: DistributedSystem.Variables)
+    {
+        && v.WF(c)
+        && Inv_ClientRequestMsg(c, v)
+        && Inv_ClientResponseMsg(c, v)
+   }
+
+    lemma RefinementInit(c: DistributedSystem.Constants, v: DistributedSystem.Variables)
+//        requires DistributedSystem.Init(c, v)
+//        ensures Inv(c, v)
+//        ensures Spec.Init(ConstantsAbstraction(c), VariablesAbstraction(c, v))
+    {
+    }
+
+    lemma RefinementNext(c: DistributedSystem.Constants, v: DistributedSystem.Variables, v': DistributedSystem.Variables, evt: Option<Host.Spec.Event>, step: DistributedSystem.Step)
+//        requires DistributedSystem.NextStep(c, v, v', evt, step)
+//        requires Inv(c, v)
+//        ensures Inv(c, v') 
+//        ensures Spec.Next(ConstantsAbstraction(c), VariablesAbstraction(c, v), VariablesAbstraction(c, v'), evt) || (VariablesAbstraction(c, v) == VariablesAbstraction(c, v') && evt == NoOp)
+    {
+    }
+}
