working/composition/event_based_refinement/load_balancer/compositional/client_server/ClientServerNetwork.t.dfy
@@ -1,0 +1,57 @@
+//include "../shared/Types.t.dfy"
+//include "../shared/Network.t.dfy"
+include "../abstract_composition/ComposedNetwork.t.dfy"
+include "../client/ClientHost.v.dfy"
+include "../server/ServerHost.v.dfy"
+
+module ClientServerNetwork refines ComposedNetwork {
+    //import opened Types
+    import HostA = ClientHost
+    import HostB = ServerHost
+    import NetworkA = ClientHost.Network
+    import NetworkB = ServerHost.Network
+
+    ghost predicate TranslateAToB(msgA: NetworkA.Message, msgB: NetworkB.Message)
+    {
+        && msgA.ClientRequest?
+        && msgB.ServerRequest?
+        && msgA.request == msgB.request
+    }
+
+    ghost predicate TranslateBToA(msgB: NetworkB.Message, msgA: NetworkA.Message)
+    {
+        && msgB.ServerResponse?
+        && msgA.ClientResponse?
+        && msgB.response == msgA.response
+    }
+
+    /*datatype Message = MessageClient(msgClient: ClientNetwork.Message) | MessageServer(msgServer: ServerNetwork.Message)
+    datatype MessageOps = MessageOps(recv:Option<Message>, send:Option<Message>)
+    datatype ComposedMessageOps = ComposedMessageOps(msgOps: MessageOps, translated: Option<Message>)
+
+    datatype Constants = Constants 
+
+    datatype Variables = Variables(sentMsgs:set<Message>)
+
+    ghost predicate Init(c: Constants, v: Variables)
+    {
+        && v.sentMsgs == {}
+    }
+
+    // todo - feels like these belong somewhere else?
+
+    ghost predicate Translate(fromMsg: Option<Message>, toMsg: Option<Message>) {
+        match (fromMsg, toMsg)
+        case (Some(MessageClient(_)), Some(MessageServer(_))) => TranslateClientToServer(fromMsg.value.msgClient, toMsg.value.msgServer)
+        case (Some(MessageServer(_)), Some(MessageClient(_))) => TranslateServerToClient(fromMsg.value.msgServer, toMsg.value.msgClient)
+        case _ => false
+    }
+
+    ghost predicate Next(c: Constants, v: Variables, v': Variables, msgOps: ComposedMessageOps) {
+        && (msgOps.msgOps.recv.Some? ==> msgOps.msgOps.recv.value in v.sentMsgs)
+        && v'.sentMsgs == v.sentMsgs
+        + (if msgOps.msgOps.send.None? then {} else { msgOps.msgOps.send.value })
+        + (if Translate(msgOps.msgOps.send, msgOps.translated) then { msgOps.translated.value } else { })
+    }
+    */
+}
