working/composition/event_based_refinement/load_balancer/compositional/client_server/ClientServerSpec.t.dfy
@@ -1,0 +1,27 @@
+include "../abstract_composition/ComposedSpec.t.dfy"
+include "../client/ClientHost.v.dfy"
+include "../server/ServerHost.v.dfy"
+
+module ClientServerSpec refines ComposedSpec {
+    import HostA = ClientHost
+    import HostB = ServerHost
+    import SpecA = ClientHost.Spec
+    import SpecB = ServerHost.Spec
+
+    /*datatype Event = EventClient(evtClient: ClientSpec.Event) | EventServer(evtServer: ServerSpec.Event)
+
+    datatype Constants = Constants(cnstsClient: ClientSpec.Constants, cnstsServer: ServerSpec.Constants)
+    datatype Variables = Variables(varsClient: ClientSpec.Variables, varsServer: ServerSpec.Variables)
+
+    ghost predicate Init(c: Constants, v: Variables) {
+        && ClientSpec.Init(c.cnstsClient, v.varsClient)
+        && ServerSpec.Init(c.cnstsServer, v.varsServer)
+    }
+
+    ghost predicate Next(c: Constants, v: Variables, v': Variables, evt: Event) {
+        match evt 
+        case EventClient(_) => ClientSpec.Next(c.cnstsClient, v.varsClient, v'.varsClient, evt.evtClient) && v.varsServer == v'.varsServer
+        case EventServer(_) => ServerSpec.Next(c.cnstsServer, v.varsServer, v'.varsServer, evt.evtServer) && v.varsClient == v'.varsClient
+    }
+    */
+}
