working/composition/event_based_refinement/load_balancer/compositional/server/DistributedSystem.v.dfy
@@ -1,0 +1,6 @@
+include "../shared/DistributedSystem.t.dfy"
+include "ServerHost.v.dfy"
+
+module DistributedSystem refines AbstractDistributedSystem {
+    import opened Host = ServerHost
+}
