working/composition/event_based_refinement/load_balancer/compositional/server/Network.v.dfy
@@ -1,0 +1,6 @@
+include "ServerSpec.t.dfy"
+include "../shared/Network.t.dfy"
+
+module ServerNetwork refines AbstractNetwork {
+    datatype Message = ServerRequest(request: ServiceRequest<(int, int)>) | ServerResponse(response: ServiceResponse<int>)
+}
