working/composition/event_based_refinement/load_balancer/compositional/server/RefinementProof.v.dfy
@@ -1,0 +1,62 @@
+include "../shared/RefinementObligation.t.dfy"
+include "ServerHost.v.dfy"
+include "Network.v.dfy"
+include "DistributedSystem.v.dfy"
+
+module RefinementProof refines RefinementTheorem {
+    import opened DistributedSystem = DistributedSystem
+
+    ghost function ConstantsAbstraction(c: DistributedSystem.Constants) : Host.Spec.Constants
+//        requires c.WF()
+    {
+        Host.Spec.Constants()
+    }
+
+    ghost function MapLog(requests: seq<ServiceRequest<(int, int)>>, responses: seq<ServiceResponse<int>>) : seq<(int, int, int)>
+        decreases |requests|
+        requires |requests| == |responses|
+        ensures |requests| == |MapLog(requests, responses)|
+        ensures forall i :: 0 <= i < |requests| ==> MapLog(requests, responses)[i] == (requests[i].val.0, requests[i].val.1, responses[i].val)
+    {
+        if |requests| == 0
+            then [] 
+            else [(requests[0].val.0, requests[0].val.1, responses[0].val)] + MapLog(requests[1..], responses[1..])
+    }
+
+    ghost function VariablesAbstraction(c: DistributedSystem.Constants, v: DistributedSystem.Variables) : Host.Spec.Variables
+//        requires v.WF(c)
+    {
+        Host.Spec.Variables(MapLog(v.hosts[0].requests, v.hosts[0].responses))
+    }
+
+    ghost predicate Inv_ServerResponseMsg(c: DistributedSystem.Constants, v: DistributedSystem.Variables) 
+        requires v.WF(c)
+    {
+        forall msg :: 
+            && msg in v.network.sentMsgs 
+            && msg.ServerResponse? ==> 
+            && |v.hosts[0].responses| > msg.response.seqNo 
+            && v.hosts[0].responses[msg.response.seqNo] == msg.response
+    }
+
+    ghost predicate Inv(c: DistributedSystem.Constants, v: DistributedSystem.Variables)
+    {
+        && v.WF(c)
+        && Inv_ServerResponseMsg(c, v)
+   }
+
+    lemma RefinementInit(c: DistributedSystem.Constants, v: DistributedSystem.Variables)
+//        requires DistributedSystem.Init(c, v)
+//        ensures Inv(c, v)
+//        ensures Spec.Init(ConstantsAbstraction(c), VariablesAbstraction(c, v))
+    {
+    }
+
+    lemma RefinementNext(c: DistributedSystem.Constants, v: DistributedSystem.Variables, v': DistributedSystem.Variables, evt: Option<Host.Spec.Event>, step: DistributedSystem.Step)
+//        requires DistributedSystem.NextStep(c, v, v', evt, step)
+//        requires Inv(c, v)
+//        ensures Inv(c, v') 
+//        ensures Spec.Next(ConstantsAbstraction(c), VariablesAbstraction(c, v), VariablesAbstraction(c, v'), evt) || (VariablesAbstraction(c, v) == VariablesAbstraction(c, v') && evt == NoOp)
+    {
+    }
+}
