working/composition/event_based_refinement/load_balancer/compositional/server/ServerSpec.t.dfy
@@ -1,0 +1,25 @@
+include "../shared/Spec.t.dfy"
+
+module ServerSpec refines AbstractSpec {
+    datatype Event = Compute
+
+    datatype Constants = Constants
+
+    datatype Variables = Variables(log: seq<(int, int, int)>)
+
+    ghost predicate Init(c: Constants, v: Variables) {
+        && |v.log| == 0
+    }
+
+    ghost predicate Compute(c: Constants, v: Variables, v': Variables) {
+        && |v'.log| == |v.log| + 1
+        && v'.log[..|v'.log| - 1] == v.log
+        && v'.log[|v'.log| - 1].2 == v'.log[|v'.log| - 1].0 + v'.log[|v'.log| - 1].1
+    }
+
+    ghost predicate Next(c: Constants, v: Variables, v': Variables, evt: Event) {
+        match evt {
+            case Compute => Compute(c, v, v')
+        }
+    }
+}
