working/composition/event_based_refinement/load_balancer/compositional/shared/Host.t.dfy
@@ -1,0 +1,23 @@
+include "Types.t.dfy"
+include "Spec.t.dfy"
+include "Network.t.dfy"
+
+abstract module AbstractHost {
+    import opened Types
+    import opened Spec: AbstractSpec
+    import Network: AbstractNetwork
+
+    type Constants {
+        ghost predicate WF()
+    }
+
+    type Variables {
+        ghost predicate WF(c: Constants)
+    }
+
+    ghost predicate GroupWFConstants(c: seq<Constants>)
+    ghost predicate GroupWFVariables(c: seq<Constants>, v: seq<Variables>)
+
+    ghost predicate Init(c: Constants, v: Variables)
+    ghost predicate Next(c: Constants, v: Variables, v': Variables, evt: Option<Spec.Event>, msgOps: Network.MessageOps)
+}
