working/composition/event_based_refinement/load_balancer/compositional/shared/RefinementObligation.t.dfy
@@ -1,0 +1,27 @@
+include "Types.t.dfy"
+include "Host.t.dfy"
+include "DistributedSystem.t.dfy"
+
+abstract module RefinementTheorem {
+    import opened Types
+    import opened DistributedSystem: AbstractDistributedSystem
+
+    ghost function ConstantsAbstraction(c: DistributedSystem.Constants) : Host.Spec.Constants
+        requires c.WF()
+
+    ghost function VariablesAbstraction(c: DistributedSystem.Constants, v: DistributedSystem.Variables) : Host.Spec.Variables
+        requires v.WF(c)
+
+    ghost predicate Inv(c: DistributedSystem.Constants, v: DistributedSystem.Variables)
+
+    lemma RefinementInit(c: DistributedSystem.Constants, v: DistributedSystem.Variables)
+        requires DistributedSystem.Init(c, v)
+        ensures Inv(c, v)
+        ensures Host.Spec.Init(ConstantsAbstraction(c), VariablesAbstraction(c, v))
+    
+    lemma RefinementNext(c: DistributedSystem.Constants, v: DistributedSystem.Variables, v': DistributedSystem.Variables, evt: Option<Host.Spec.Event>, step: DistributedSystem.Step)
+        requires DistributedSystem.NextStep(c, v, v', evt, step)
+        requires Inv(c, v)
+        ensures Inv(c, v') 
+        ensures (evt.Some? && Host.Spec.Next(ConstantsAbstraction(c), VariablesAbstraction(c, v), VariablesAbstraction(c, v'), evt.value)) || (evt.None? && VariablesAbstraction(c, v) == VariablesAbstraction(c, v'))
+}
