working/composition/event_based_refinement/load_balancer/compositional/shared/Spec.t.dfy
@@ -1,0 +1,13 @@
+include "Types.t.dfy"
+
+abstract module AbstractSpec {
+    import opened Types
+    
+    type Event
+
+    type Constants
+    type Variables
+
+    ghost predicate Init(c: Constants, v: Variables)
+    ghost predicate Next(c: Constants, v: Variables, v': Variables, evt: Event)
+}
