working/composition/event_based_refinement/load_balancer/compositional/shared/Types.t.dfy
@@ -1,0 +1,8 @@
+module Types {
+    datatype Option<T> = Some(value:T) | None
+
+    type SeqNo = nat
+
+    datatype ServiceRequest<T> = ServiceRequest(seqNo: SeqNo, val: T)
+    datatype ServiceResponse<T> = ServiceResponse(seqNo: SeqNo, val: T)
+}
