working/composition/event_based_refinement/load_balancer/monolithic/AdditionServiceSpec.t.dfy
@@ -1,0 +1,53 @@
+module Types {
+    datatype Option<T> = Some(value:T) | None
+
+    datatype Event = SendRequest | ReceiveResponse | NoOp
+
+    type SeqNo = nat
+
+    datatype ClientRequest = ClientRequest(seqNo: SeqNo, x: int, y: int)
+    datatype ClientResponse = ClientResponse(seqNo: SeqNo, sum: int)
+
+    datatype Message =
+    | ClientRequestMsg(request: ClientRequest)
+    | LBRequestMsg(request: ClientRequest)
+    | LBResponseMsg(response: ClientResponse)
+    | ClientResponseMsg(response: ClientResponse)
+
+    datatype MessageOps = MessageOps(recv:Option<Message>, send:Option<Message>)
+}
+
+module Spec {
+    import opened Types
+
+    datatype Constants = Constants
+
+    datatype Variables = Variables(nums: seq<(int, int)>, sum: seq<int>)
+
+    ghost predicate Init(c: Constants, v: Variables) {
+        && |v.nums| == 0
+        && |v.sum| == 0
+    }
+
+    ghost predicate SendRequest(c: Constants, v: Variables, v': Variables) {
+        && |v'.nums| == |v.nums| + 1
+        && v'.nums[..|v'.nums| - 1] == v.nums
+        && v.sum == v'.sum
+    }
+
+    ghost predicate ReceiveResponse(c: Constants, v: Variables, v': Variables) {
+        && v.nums == v'.nums
+        && |v.sum| < |v.nums|
+        && |v'.sum| == |v.sum| + 1
+        && v'.sum[..|v'.sum| - 1] == v.sum
+        && v'.sum[|v'.sum| - 1] == v.nums[|v'.sum| - 1].0 + v.nums[|v'.sum| - 1].1
+    }
+
+    ghost predicate Next(c: Constants, v: Variables, v': Variables, evt: Event) {
+        match evt {
+            case SendRequest => SendRequest(c, v, v')
+            case ReceiveResponse => ReceiveResponse(c, v, v')
+            case NoOp => v == v'
+        }
+    }
+}
